feat: add cbv annotations to iterators, ranges and string definitions

src/Init/Data/List/Basic.lean
@@ -1246,6 +1246,22 @@ def IsInfix (l₁ : List α) (l₂ : List α) : Prop := Exists fun s => Exists f
 /-- not `isInfix` -/
 recommended_spelling "infix" for "<:+:" in [IsInfix, «term_<:+:_»]
 
+/--
+Checks whether the first list is a contiguous sub-list of the second.
+
+The relation `List.IsInfixOf` expresses this property with respect to logical equality.
+
+Examples:
+ * `[2, 3].isInfixOf [1, 2, 3, 4] = true`
+ * `[2, 3].isInfixOf [1, 3, 2, 4] = false`
+ * `[2, 3].isInfixOf [2, 3] = true`
+ * `[2, 3].isInfixOf [1] = false`
+-/
+def isInfixOf [BEq α] (l₁ l₂ : List α) : Bool :=
+  l₁.isPrefixOf l₂ || match l₂ with
+    | []      => false
+    | _ :: l₂ => isInfixOf l₁ l₂
+
 /-! ### splitAt -/
 
 /--
