src/Init/Data/String/Lemmas/Modify.lean
@@ -49,6 +49,11 @@ theorem toList_mapAux {f : Char → Char} {s : String} {p : s.Pos}
 theorem toList_map {f : Char → Char} {s : String} : (s.map f).toList = s.toList.map f := by
   simp [map, toList_mapAux s.splits_startPos]
 
+@[cbv_eval]
+theorem map_eq {f : Char → Char} {s : String} : s.map f = .ofList (s.toList.map f) := by
+  apply String.toList_injective
+  simp only [toList_map, toList_ofList]
+
 @[simp]
 theorem length_map {f : Char → Char} {s : String} : (s.map f).length = s.length := by
   simp [← length_toList]
